compiler/bootstrap/compilation/x64/64/x64BootstrapScript.sml
@@ -1,11 +1,16 @@
 (*
-  Evaluateof the 64-bit version of the compiler into x64 machine code.
+  Evaluate the 64-bit version of the compiler into x64 machine code.
 *)
 open preamble compiler64ProgTheory eval_cake_compile_x64Lib;
 
 val _ = new_theory "x64Bootstrap"
 
 Theorem compiler64_compiled =
-  eval_cake_compile_x64 "" compiler64_prog_def "cake.S";
+  eval_cake_compile_x64_general
+    { prefix               = ""
+    , conf_def             = x64_configTheory.x64_backend_config_def
+    , prog_def             = compiler64_prog_def
+    , output_filename      = "cake.S"
+    , output_conf_filename = SOME "config_enc_str.txt" };
 
 val _ = export_theory ();
