examples/lpr_checker/array/compilation/lpr_arrayCompileARM8Script.sml
@@ -1,11 +1,11 @@
 (*
   Compiles the lpr example by evaluation inside the logic of HOL
 *)
-open preamble compilationLib lpr_arrayFullProgTheory
+open preamble lpr_arrayFullProgTheory eval_cake_compile_arm8Lib
 
 val _ = new_theory "lpr_arrayCompileARM8"
 
-val lpr_array_compiled = save_thm("lpr_array_compiled",
-  compile_arm8 "cake_lpr_arm8" check_unsat_prog_def);
+Theorem lpr_array_compiled =
+  eval_cake_compile_arm8 "" check_unsat_prog_def "cake_lpr_arm8.S";
 
 val _ = export_theory ();
