examples/opentheory/compilation/ag32/proofs/readerProgProofScript.sml
@@ -70,7 +70,7 @@ val reader_startup_clock_def =
   |> SIMP_RULE bool_ss [GSYM RIGHT_EXISTS_IMP_THM,SKOLEM_THM]);
 
 val compile_correct_applied =
-  MATCH_MP compile_correct reader_compiled
+  MATCH_MP compile_correct (cj 1 reader_compiled)
   |> SIMP_RULE(srw_ss())[LET_THM,ml_progTheory.init_state_env_thm,GSYM AND_IMP_INTRO]
   |> C MATCH_MP reader_not_fail
   |> C MATCH_MP ag32_backend_config_ok
