tutorial/wordfreqCompileScript.sml
@@ -2,12 +2,11 @@
   Compile the wordfreq program to machine code by evaluation of the compiler in
   the logic.
 *)
-
-open preamble wordfreqProgTheory compilationLib
+open preamble wordfreqProgTheory eval_cake_compile_x64Lib
 
 val _ = new_theory"wordfreqCompile";
 
-val wordfreq_compiled = save_thm("wordfreq_compiled",
-  compile_x64 "wordfreq" wordfreq_prog_def);
+Theorem wordfreq_compiled =
+  eval_cake_compile_x64 "" wordfreq_prog_def "wordfreq.S";
 
 val _ = export_theory();
